src/Imps/Imp/Syntax.v
@@ -1,5 +1,3 @@
-From Stdlib Require Export Recdef.
-
 From FormalSystems Require Export Base.
 
 Inductive AExp : Type :=
@@ -25,7 +23,7 @@ Definition State : Type := Loc -> nat.
 Definition initialState : State := fun _ => 0.
 
 Definition changeState (s : State) (x : Loc) (n : nat) : State :=
-  fun y : Loc => if x =? y then n else s y.
+  fun y : Loc => if decide (x = y) then n else s y.
 
 Fixpoint loca (a : AExp) : list Loc :=
 match a with
